Got rid of state_wf, updated ticketlock model

fairness/examples/ticketlock/ticketlock_model.v
@@ -30,22 +30,29 @@ Section Model.
 
   Let tl_role_map := gmap tl_role tl_role_st. 
 
-  Record tl_st := mkTlSt {
-                      owner: nat;
-                      ticket: nat;
-                      role_map: tl_role_map;
-                    }. 
+  Definition tl_st' := (nat * nat * tl_role_map)%type. 
 
   Definition tl_state_wf
-    '(mkTlSt o t rm) :=
+    (st': tl_st'): Prop :=
+    let '(o, t, rm) := st' in
     (* (o t: nat) (rm: tl_role_map) := *)
     o <= t /\
     (forall k, o <= k < t <-> exists ρ e, rm !! ρ = Some (tl_U k, e)) /\
     (forall ρ k, rm !! ρ = Some (tl_U k, false) -> k = o) /\
     (forall ρ1 ρ2 k e1 e2 (R1: rm !! ρ1 = Some (tl_U k, e1))
        (R2: rm !! ρ2 = Some (tl_U k, e2)), ρ1 = ρ2).
+
     
-  Notation "<{ o , t , rm }>" := (mkTlSt o t rm).
+  Record tl_st := mkTlSt {
+                      owner: nat;
+                      ticket: nat;
+                      role_map: tl_role_map;
+                      tl_wf: tl_state_wf (owner, ticket, role_map);
+                    }. 
+
+  Definition simpl_tl_st '(mkTlSt o t rm wf): tl_st' := (o, t, rm). 
+
+  Notation "<{ o , t , rm }>" := (o, t, rm).
 
   #[global] Instance tl_role_eqdec: EqDecision tl_role.
   Proof using. solve_decision. Qed. 
@@ -56,13 +63,18 @@ Section Model.
   #[global] Instance tl_role_st_eqdec: EqDecision tl_role_st. 
   Proof using. solve_decision. Qed. 
 
+  Instance wf_PI st': ProofIrrel (tl_state_wf st').
+  Proof. apply make_proof_irrel. Qed. 
+
   #[global] Instance tl_st_eqdec: EqDecision tl_st. 
   Proof using.
-    solve_decision.
+    intros [o1 t1 rm1 wf1] [o2 t2 rm2 wf2].
+    destruct (decide (o1 = o2 /\ t1 = t2 /\ rm1 = rm2)).
+    2: { right. set_solver. }
+    destruct a as (->&->&->).
+    left. eapply @f_equal. apply wf_PI.  
   Qed. 
 
-  (* Definition tl_st_wf := { st | tl_state_wf st}. *)
-    
   Lemma role_of_dec (rm: tl_role_map) (s: tl_role_st):
     {r | rm !! r = Some s} + (forall r, rm !! r ≠ Some s). 
   Proof using.
@@ -76,25 +88,31 @@ Section Model.
     apply map_filter_lookup_Some in IN. destruct IN as [IN <-]. eauto.
   Qed.  
 
-  Let advance_next (st: tl_st) := 
-        match role_of_dec (role_map st) (tl_U (owner st), true) with
+  (* Let advance_next (o t: nat) rm :=  *)
+  Let advance_next: tl_st' -> tl_st' :=
+        fun '(o, t, rm) =>
+        match role_of_dec rm (tl_U o, true) with
         | inl (exist _ r _) => 
-            let rm' := <[r := (tl_U (owner st), false)]> (role_map st) in
-            mkTlSt (owner st) (ticket st) rm'
-        | inr NO => st
+            let rm' := <[r := (tl_U o, false)]> rm in
+            (* mkTlSt (owner st) (ticket st) rm' *)
+            (o, t, rm')
+        | inr NO => (o, t, rm)
         end.
 
-  Inductive tl_trans: tl_st -> option tl_role -> tl_st -> Prop :=
+  Inductive tl_trans': tl_st' -> option tl_role -> tl_st' -> Prop :=
   | tl_take_ticket o t rm r (R: rm !! r = Some (tl_L, true)):
     let next_en := if decide (o = t) then false else true in
-    tl_trans <{o, t, rm}> (Some r) <{o, t + 1, <[r := (tl_U t, next_en)]> rm}>
+    tl_trans' <{o, t, rm}> (Some r) <{o, t + 1, <[r := (tl_U t, next_en)]> rm}>
   | tl_spin (o t k: nat) rm r (LT: o ≠ k) (R: rm !! r = Some (tl_U k, true)):
-    tl_trans <{o, t, rm}> (Some r) <{o, t, rm}>
+    tl_trans' <{o, t, rm}> (Some r) <{o, t, rm}>
   | tl_unlock o t rm r (R: rm !! r = Some (tl_U o, true)):
     let st' := <{o + 1, t, <[r := (tl_L, false)]> rm}> in
     let st'' := advance_next st' in
-    tl_trans <{o, t, rm}> (Some r) st''
+    tl_trans' <{o, t, rm}> (Some r) st''
   .
+
+  Definition tl_trans st1 oρ st2 :=
+    tl_trans' (simpl_tl_st st1) oρ (simpl_tl_st st2). 
 
   Definition tl_live_roles (st: tl_st): gset tl_role :=
     dom (filter (fun '(r, (_, e)) => e = true) (role_map st)).
@@ -103,12 +121,33 @@ Section Model.
     forall s ρ s', tl_trans s (Some ρ) s' -> ρ ∈ tl_live_roles s.
   Proof.
     intros s ρ s' TRANS. rewrite /tl_live_roles.
+    destruct s, s'. 
     inversion TRANS; subst; simpl. 
     all: eapply elem_of_dom_2; apply map_filter_lookup_Some_2; done.
   Qed.
 
+  Definition tl_init_st' (n: nat): tl_st' :=
+    let rm := gset_to_gmap (tl_L, true) (set_seq 0 n) in
+    <{ 0, 0, rm }>.
+
+  Lemma tl_init_st'_wf n:
+    tl_state_wf (tl_init_st' n). 
+  Proof using. 
+    rewrite /tl_init_st'. 
+    red. split; [lia| ]. split; [| split]. 
+    - split; [lia| ]. intros [ρ [? RMρ]].
+      apply lookup_gset_to_gmap_Some in RMρ as [_ ?]. congruence.
+    - intros. rewrite lookup_gset_to_gmap_Some in H.
+      by destruct H. 
+    - intros. rewrite lookup_gset_to_gmap_Some in R1. 
+      by destruct R1.
+  Qed. 
+  
   #[global] Instance tlSt_inhabited: Inhabited tl_st. 
-  Proof. exact (populate (mkTlSt 0 0 ∅)). Qed.
+  Proof.
+    apply populate. esplit.
+    apply (tl_init_st'_wf 0).
+  Qed. 
 
   Definition tl_fair_model: FairModel.
   Proof.
@@ -131,17 +170,244 @@ Section Model.
   Definition active_st (ρ: tl_role) (st: tl_st) :=
     exists r, (role_map st) !! ρ = Some (r, true).
 
+
+  Ltac simpl_li_eq := match goal with
+                      | H: <[?x:=?y]> ?m !! ?x = ?r |- _
+                        => rewrite lookup_insert in H
+                      end.
+  Ltac simpl_li_eq' := match goal with
+                       | |- <[?x:=?y]> ?m !! ?x = ?r
+                         => rewrite lookup_insert
+                       end.
+  
+  Ltac simpl_li_neq := match goal with
+                       | H: <[?x:=?y]> ?m !! ?x' = ?r, NE: ?x ≠ ?x' |- _ => 
+                           rewrite lookup_insert_ne in H; [| by apply NE]
+                       | H: <[?x:=?y]> ?m !! ?x' = ?r, NE: ?x' ≠ ?x |- _ =>
+                           rewrite lookup_insert_ne in H;
+                           [| by apply not_eq_sym; apply NE]
+                       end.
+  Ltac simpl_li_neq' := match goal with
+                        | NE: ?x ≠ ?x' |- <[?x:=?y]> ?m !! ?x' = ?r => 
+                            rewrite lookup_insert_ne; [| by apply NE]
+                        | NE: ?x' ≠ ?x |- <[?x:=?y]> ?m !! ?x' = ?r => 
+                            rewrite lookup_insert_ne;
+                            [| by apply not_eq_sym; apply NE]
+                        end.
+  
+  Ltac simpl_li := (repeat simpl_li_eq); (repeat simpl_li_neq);
+                   (try simpl_li_eq'); (try simpl_li_neq'). 
+
+
+  Lemma advance_next_helper_U o t (rm: tl_role_map) ρo ρ k b
+    (RMρo: rm !! ρo = Some (tl_U o, true))
+    (UNIQ: forall ρ1 ρ2 k e1 e2 (R1: rm !! ρ1 = Some (tl_U k, e1))
+             (R2: rm !! ρ2 = Some (tl_U k, e2)), ρ1 = ρ2)
+    (TKo: forall ρ k, rm !! ρ = Some (tl_U k, false) -> k = o):
+    snd (advance_next (<{o + 1, t, <[ρo := (tl_L, false)]> rm}>)) !! ρ = Some (tl_U k, b) <-> (exists b', rm !! ρ = Some (tl_U k, b') /\
+                 (k = o + 1 /\ b = false /\ b' = true \/
+                  k ≠ o /\ k ≠ (o + 1) /\ b' = b)). 
+  Proof using.
+    rewrite /advance_next.
+    destruct role_of_dec as [[? ?] | ?]; simpl in *.
+    - assert (x ≠ ρo) as NEQ.
+      { intros ->. rewrite lookup_insert in e. congruence. }
+      rewrite lookup_insert_ne in e; auto.
+      destruct (decide (x = ρ)) as [-> | NEQ'].
+      { rewrite lookup_insert. split.
+        - intros. inversion H. eexists. eauto.
+        - intros [b' [RMρ ST]].
+          rewrite e in RMρ. intuition; congruence. }
+      rewrite lookup_insert_ne; auto.
+      destruct (decide (ρo = ρ)) as [-> | NEQ''].
+      { rewrite lookup_insert. rewrite RMρo. split; intros ST. 
+        - congruence.
+        - destruct ST as [b' ST]; intuition; subst.
+          + inversion H. lia.
+          + congruence. }
+      rewrite lookup_insert_ne; auto. split; intros; intuition. 
+      + exists b. split; auto. right. repeat split; auto; intros ->.
+        * destruct NEQ''. eapply UNIQ; eauto.
+        * destruct NEQ'. eapply UNIQ; eauto.
+      + destruct H as [b' [X ?]]. rewrite X.
+        repeat f_equal. intuition. subst.  
+        destruct NEQ'. eapply UNIQ; eauto. 
+    - destruct (decide (ρo = ρ)) as [-> | NEQ''].
+      { rewrite /advance_next. rewrite lookup_insert.
+        rewrite RMρo. split; intros; intuition; try congruence.
+        destruct H as [? [? [?|?]]]; subst.
+        - inversion H. lia.
+        - intuition. congruence. }
+      rewrite lookup_insert_ne; auto. split; intros; intuition; auto.
+      + exists b. split; auto. right. repeat split; auto. 
+        * intros ->. destruct NEQ''; eapply UNIQ; eauto.
+        * intros ->. destruct b.
+          ** destruct (n ρ). rewrite lookup_insert_ne; auto.
+          ** apply TKo in H. lia.
+      + destruct H as [? [? ?]]; intuition; subst; auto.
+        destruct (n ρ). rewrite lookup_insert_ne; auto.
+  Qed. 
+  
+  Lemma step_preserves_tl_state_wf st ℓ st'
+    (WF: tl_state_wf st) (STEP: tl_trans' st ℓ st'):
+    tl_state_wf st'.
+  Proof using. 
+    destruct st as [[o t] rm]. destruct st' as [[o' t'] rm'].
+    red in WF. destruct WF as (LE & TKS & TKo & UNIQ).
+    inversion STEP; subst; simpl in *; auto.
+    + rename o' into o.
+      split; [lia| ]. 
+      split; [| split]. 
+      * intros. specialize (TKS k).
+        destruct (decide (k = t)) as [-> | NEQ].
+        { split; [| lia]. intros T.
+          exists r. eexists. rewrite lookup_insert. split; eauto. }
+        etransitivity.
+        { etransitivity; [| apply TKS]. lia. }
+        split; intros; intuition. 
+        ** destruct H as (?&?&?). 
+           do 2 eexists. rewrite lookup_insert_ne; eauto.
+           intros <-. congruence.
+        ** destruct H as (?&?&?).
+           do 2 eexists.
+           rewrite <- H. symmetry. apply lookup_insert_ne.
+           intros <-. rewrite lookup_insert in H. congruence.
+      * intros.
+        destruct (decide (r = ρ)) as [-> | NEQ].
+        2: { rewrite lookup_insert_ne in H; eauto. } 
+        rewrite lookup_insert in H. inversion H.
+        subst k next_en0.
+        destruct (decide (o = t)); congruence.
+      * intros. destruct (decide (ρ1 = r)), (decide (ρ2 = r)).
+        all: subst; simpl_li; inversion R1; inversion R2; subst; auto. 
+        1, 2: enough (k < k); [lia| ]; apply TKS; by eauto.
+        eapply UNIQ; eauto.
+    + subst st'' st'2 st'1 st'0 st'.
+      assert (o' = o + 1 /\ t' = t) as [-> ->].
+      { rewrite /advance_next in H.
+        destruct (role_of_dec _ _) as [[? ?] | ?]; by inversion H. }
+      apply Nat.le_lteq in LE as [LT | ->].
+      2: { enough (t < t); [lia| ]. apply TKS. eauto. }
+      rewrite H. red.
+      split; [lia| ]. split; [| split]. 
+      * intros. 
+        rewrite /advance_next in H.
+        destruct (role_of_dec) as [[? ?] | ?]; simpl in *;
+          inversion H; subst rm'; clear H.
+        ** destruct (decide (r = x)).
+           { subst x. rewrite lookup_insert in e. congruence. }
+           rewrite lookup_insert_ne in e; auto.
+           destruct (decide (k = o)) as [-> | NEQ].
+           { split; [lia| ]. intros (ρ' & e' & RMρ'). 
+             destruct (decide (ρ' = r)).
+             { subst ρ'. rewrite lookup_insert_ne in RMρ'; auto.
+               rewrite lookup_insert in RMρ'. congruence. }
+             destruct (decide (x = ρ')).
+             { subst x. rewrite lookup_insert in RMρ'.
+               inversion RMρ'. lia. }
+             rewrite !lookup_insert_ne in RMρ'; auto.
+             destruct n0. eapply UNIQ; eauto. }
+           etransitivity; [etransitivity| ]; [| by apply (TKS k) |].
+           { lia. }
+           split.
+           *** intros. destruct H as (?&?&?). 
+               destruct (decide (k = o + 1)).
+               **** subst. exists x, false. by rewrite lookup_insert.
+               **** do 2 eexists. 
+                    rewrite !lookup_insert_ne; [by apply H| ..].
+                    { congruence. }
+                    intros <-. rewrite e in H. congruence.
+           *** intros. destruct H as (?&?&?). 
+               destruct (decide (k = o + 1)).
+               **** subst. eauto.
+               **** destruct (decide (x = x0)).
+                    all: subst; simpl_li; inversion H; subst.
+                    { lia. }
+                    destruct (decide (r = x0)). 
+                    all: subst; simpl_li; inversion H; subst; eauto. 
+        ** specialize (TKS k). 
+           split.
+           *** intros [GEk LTk].
+               apply proj1 in TKS.
+               specialize_full TKS; [lia| ]. destruct TKS as (?&?&TKS). 
+               do 2 eexists. rewrite lookup_insert_ne; eauto.
+               intros <-. rewrite R in TKS.
+               inversion TKS. lia.
+           *** intros. destruct H as (?&?&H). 
+               destruct (decide (r = x)) as [-> | ?].
+               { rewrite lookup_insert in H. congruence. }
+               destruct (decide (k = o)) as [-> | NEQko].
+               **** rewrite lookup_insert_ne in H; auto. 
+                    destruct n0. eapply UNIQ; eauto. 
+               **** enough (o <= k < t); [lia| ]. apply TKS.
+                    rewrite lookup_insert_ne in H; eauto.
+      * intros. rewrite /advance_next in H.
+        destruct role_of_dec as [[? ?] | ?]; simpl in *; 
+          inversion H; subst rm'; clear H.
+        ** destruct (decide (r = x)), (decide (x = ρ)), (decide (r = ρ)); 
+             do 2 (subst; simpl_li; inversion H0; inversion e; subst; auto).
+           apply TKo in H0. subst k.
+           destruct n1. eapply UNIQ; eauto. 
+        ** destruct (decide (r = ρ));
+             subst; simpl_li; inversion H0; subst; auto. 
+           apply TKo in H0. subst k.
+           destruct n0. eapply UNIQ; eauto. 
+      * intros.
+        pose proof H as rm'_eq. apply (f_equal snd) in rm'_eq. simpl in rm'_eq.
+        rewrite -rm'_eq in R1 R2. 
+        eapply advance_next_helper_U in R1, R2; auto.
+        destruct R1 as (?&?&R0), R2 as (?&?&R3).
+        destruct R0, R3; intuition; subst.
+        all: lia || eapply UNIQ; eauto.
+  Qed. 
+        
+  Lemma tl_trans_reduce st1' oρ st2'
+    (TRANS': tl_trans' st1' oρ st2')
+    (WF1: tl_state_wf st1'):
+    exists st1 st2, simpl_tl_st st1 = st1' /\ simpl_tl_st st2 = st2' /\ tl_trans st1 oρ st2.
+  Proof.
+    destruct st1' as [[o1 t1] rm1], st2' as [[o2 t2] rm2].
+    pose proof (step_preserves_tl_state_wf _ _ _ WF1 TRANS') as WF2.  
+    exists (mkTlSt o1 t1 rm1 WF1), (mkTlSt o2 t2 rm2 WF2).
+    done. 
+  Qed. 
+
+  Definition enhance_tl_st' (st': tl_st') (wf: tl_state_wf st'): tl_st.
+    destruct st' as [[o t] rm].
+    eapply mkTlSt; eauto.
+  Defined. 
+
+  Lemma tl_trans_reduce' o1 t1 rm1 wf1 oρ o2 t2 rm2
+    (TRANS': tl_trans' (o1, t1, rm1) oρ (o2, t2, rm2)):
+    tl_trans (mkTlSt o1 t1 rm1 wf1) oρ (mkTlSt o2 t2 rm2 (step_preserves_tl_state_wf _ _ _ wf1 TRANS')).
+  Proof.
+    done. 
+  Qed.
+
+
+  Lemma tl_trans_reduce'' o1 t1 rm1 wf1 oρ st2'
+    (TRANS': tl_trans' (o1, t1, rm1) oρ st2'):
+    tl_trans (mkTlSt o1 t1 rm1 wf1) oρ (enhance_tl_st' st2' (step_preserves_tl_state_wf _ _ _ wf1 TRANS')). 
+  Proof.
+    destruct st2' as [[o2 t2] rm2]. done. 
+  Qed.
+
   Lemma active_st_enabled (ρ: tl_role) (st: tl_st):
     active_st ρ st <-> @role_enabled_model tl_fair_model ρ st.
   Proof using.
     destruct st as [o t rm].
-    rewrite /active_st /role_enabled_model. split.
+    rewrite /active_st. simpl. split.
     - intros [r RMρ]. destruct r.
-      + eapply fm_live_spec. apply tl_take_ticket. eauto.
+      + eapply fm_live_spec.
+        unshelve apply tl_trans_reduce'.
+        4: by apply tl_take_ticket.
       + destruct (decide (o = t0)); eapply fm_live_spec. 
-        * eapply tl_unlock; eauto. rewrite RMρ. congruence.
-        * eapply tl_spin; eauto.
-    - intros LIVE. simpl in LIVE. rewrite /tl_live_roles in LIVE.
+        * unshelve apply tl_trans_reduce''. 
+          2: { subst. eapply tl_unlock. rewrite RMρ. congruence. }
+        * unshelve apply tl_trans_reduce''.
+          2: { eapply tl_spin; eauto. }
+    - intros LIVE. red in LIVE. 
+      simpl in LIVE. rewrite /tl_live_roles in LIVE.
       apply elem_of_dom in LIVE as [r LIVE]. eauto.
       apply map_filter_lookup_Some in LIVE as [? ?].
       destruct r. subst. eauto.      
@@ -159,39 +425,143 @@ Section Model.
   Qed. 
     
 
-  Definition tl_init_st (n: nat): tl_st :=
-    let rm := gset_to_gmap (tl_L, true) (set_seq 0 n) in
-    <{ 0, 0, rm }>.
-
-  Definition tl_is_init_st (st: tl_st) := 
-    exists n, st = tl_init_st n. 
-
+  (* Definition tl_is_init_st (st: tl_st) :=  *)
+  (*   exists n, st = tl_init_st n.  *)
 
   Section TlExtTrans.
 
-    Inductive allows_unlock ρ : tl_st -> tl_st -> Prop :=
+    Inductive allows_unlock' ρ : tl_st' -> tl_st' -> Prop :=
     | allows_unlock_step o t rm (LOCK: rm !! ρ = Some (tl_U o, false)):
-      allows_unlock ρ (mkTlSt o t rm) (mkTlSt o t (<[ρ := (tl_U o, true)]> rm))
+      allows_unlock' ρ (o, t, rm) (o, t, (<[ρ := (tl_U o, true)]> rm))
     .
 
-    Inductive allows_lock ρ : tl_st -> tl_st -> Prop :=
+    Inductive allows_lock' ρ : tl_st' -> tl_st' -> Prop :=
     | allows_lock_step t o rm (LOCK: rm !! ρ = Some (tl_L, false)):
-      allows_lock ρ (mkTlSt o t rm) (mkTlSt o t (<[ρ := (tl_L, true)]> rm))
+      allows_lock' ρ (o, t, rm) (o, t, (<[ρ := (tl_L, true)]> rm))
     .
 
-    Definition allow_unlock_impl ρ '(mkTlSt o t rm) :=
-      (* let unlockers := dom (filter (fun '(_, v) => v = (tl_U o, false)) rm) in *)
-      (* let oρ := nth_error (elements unlockers) 0 in *)
-      (* let rm' := match oρ with *)
-      (*            | Some ρ => (<[ρ := (tl_U o, true)]> rm)  *)
-      (*            | None => rm *)
-      (*            end in *)
-      (* mkTlSt o t rm'.  *)
-      mkTlSt o t (<[ρ := (tl_U o, true)]> rm). 
+    Definition allows_unlock ρ st1 st2 := 
+      allows_unlock' ρ (simpl_tl_st st1) (simpl_tl_st st2). 
 
-    Definition allow_lock_impl ρ '(mkTlSt o t rm) := 
-      mkTlSt o t (<[ρ := (tl_L, true)]> rm). 
+    Definition allows_lock ρ st1 st2 := 
+      allows_lock' ρ (simpl_tl_st st1) (simpl_tl_st st2).
 
+    Lemma allows_unlock'_preserves_tl_state_wf ρ st st'
+      (STEP: allows_unlock' ρ st st')
+      (WF: tl_state_wf st):
+      tl_state_wf st'.
+    Proof.
+      destruct st as [[o t] rm]. destruct st' as [[o' t'] rm'].
+      red in WF. destruct WF as (LE & TKS & TKo & UNIQ).
+      inversion STEP; subst.
+      split; auto.
+      split; [| split]. 
+      * intros. etransitivity; [etransitivity|]; [| apply TKS |]; [reflexivity|..].
+        split; intros; intuition; destruct H as (?&?&?). 
+        ** destruct (decide (x = ρ)) as [-> | NEQ].
+           *** exists ρ, true. rewrite lookup_insert. congruence.
+           *** exists x, x0. rewrite lookup_insert_ne; auto.
+        ** destruct (decide (x = ρ)) as [-> | NEQ].
+           *** rewrite lookup_insert in H.
+               exists ρ, false. congruence.
+           *** rewrite lookup_insert_ne in H; auto.
+               eauto.
+      * intros. eapply TKo; eauto. rewrite -H.
+        symmetry. apply lookup_insert_ne.
+        intros ->. rewrite lookup_insert in H. congruence.
+      * intros.
+        destruct (decide (ρ1 = ρ)), (decide (ρ2 = ρ)).
+        all: subst; simpl_li; inversion R1; inversion R2; subst; auto. 
+        all: eapply UNIQ; eauto.
+    Qed. 
+ 
+    Lemma allows_lock'_preserves_tl_state_wf ρ st st'
+      (STEP: allows_lock' ρ st st')
+      (WF: tl_state_wf st):
+      tl_state_wf st'.
+    Proof.
+      destruct st as [[o t] rm]. destruct st' as [[o' t'] rm'].
+      red in WF. destruct WF as (LE & TKS & TKo & UNIQ).
+      inversion STEP; subst.
+      split; auto. split; [| split]. 
+      * intros. etransitivity; [etransitivity|]; [| apply TKS |]; [reflexivity|..].
+        split; intros; intuition; destruct H as (?&?&?). 
+        ** exists x, x0. destruct (decide (x = ρ)); 
+             subst; simpl_li; [congruence| auto]. 
+        ** destruct (decide (x = ρ)); subst; simpl_li; inversion H; eauto.
+      * intros. destruct (decide (ρ0 = ρ)); subst; simpl_li; try congruence.
+        eapply TKo; eauto.
+      * intros.
+        destruct (decide (ρ1 = ρ)), (decide (ρ2 = ρ)).
+        all: subst; simpl_li; inversion R1; inversion R2; subst; auto. 
+        all: eapply UNIQ; eauto.
+    Qed. 
+
+    Instance allows_lock_ex_dec:
+      forall st ρ, Decision (∃ st', allows_lock ρ st st'). 
+    Proof using.
+      intros [o t rm] ρ. rewrite /allows_lock. simpl. 
+      destruct (decide (rm !! ρ = Some (tl_L, false))).
+      - left. simpl.
+        forward eapply allows_lock_step as AL.
+        { apply e. }
+        pose proof (allows_lock'_preserves_tl_state_wf _ _ _ AL tl_wf0) as WF2.
+        exists (mkTlSt o t (<[ρ:=(tl_L, true)]> rm) WF2).
+        done. 
+      - right. intros [st' L]. inversion L. congruence. 
+    Defined.
+
+    Instance allows_unlock_ex_dec: 
+      forall st ρ, Decision (∃ st', allows_unlock ρ st st'). 
+    Proof using. 
+      intros [o t rm] ρ. rewrite /allows_unlock. simpl. 
+      destruct (decide (rm !! ρ = Some (tl_U o, false))). 
+      - left. 
+        forward eapply allows_unlock_step as AL.
+        { apply e. }
+        pose proof (allows_unlock'_preserves_tl_state_wf _ _ _ AL tl_wf0) as WF2.
+        exists (mkTlSt o t (<[ρ:=(tl_U o, true)]> rm) WF2).
+        done. 
+      - right. intros [st' TRANS]. inversion TRANS. subst. set_solver.
+    Defined.  
+
+    Definition tl_active_exts st: gset fl_EI := 
+      set_map (flU (M := tl_fair_model)) 
+          (filter (fun ρ => exists st', allows_unlock ρ st st') (dom (role_map st)))
+      ∪
+      set_map (flL (M := tl_fair_model)) 
+          (filter (fun ρ => exists st', allows_lock ρ st st') (dom (role_map st))).
+    
+    Lemma tl_active_exts_spec st ι:
+      ι ∈ tl_active_exts st <-> ∃ st', @fl_ETs tl_fair_model allows_unlock allows_lock ι st st'.
+    Proof using. 
+      destruct st as [o t rm wf]. 
+      unfold tl_active_exts.
+      rewrite elem_of_union.
+      rewrite !elem_of_map. repeat setoid_rewrite elem_of_filter.
+      simpl.  
+      erewrite exist_proper.
+      2: { intros. rewrite and_assoc. apply iff_and_impl_helper.
+           intros [? [[o2 t2 rm2 wf2] AU]]. subst.
+           red in AU. simpl in AU. inversion AU. subst.  
+           by eapply elem_of_dom. }
+      rewrite or_comm. 
+      erewrite exist_proper.
+      2: { intros. rewrite and_assoc. apply iff_and_impl_helper.
+           intros [? [[o2 t2 rm2 wf2] AU]]. subst.
+           red in AU. simpl in AU. inversion AU. subst.  
+           by eapply elem_of_dom. }
+      destruct ι; set_solver. 
+    Qed. 
+
+    Global Instance tl_FLE: FairLockExt tl_fair_model.
+    esplit.
+    apply tl_active_exts_spec.
+    Defined. 
+    
+    Instance ExtTL: ExtModel tl_fair_model := 
+      FL_EM tl_FLE. 
+    
     (* TODO: move*)
     Lemma lookup_empty_dom:
   ∀ {K : Type} {M : Type → Type} {D : Type} {H : ∀ A : Type, Dom (M A) D} 
@@ -210,117 +580,11 @@ Section Model.
       apply map_choose in n as (?&?&n). by rewrite ALL in n.
     Qed.
 
-
-    Lemma allows_unlock_impl_spec ρ st (WF: tl_state_wf st):
-      forall st', allows_unlock ρ st st' <-> 
-              (allow_unlock_impl ρ st = st' /\ (has_lock_st ρ st /\ ¬ active_st ρ st)).
-    Proof.
-      destruct st as [o t rm]. intros [o' t' rm'].
-      rewrite /allow_unlock_impl /has_lock_st /active_st. simpl.  
-      destruct (rm !! ρ) as [[s e] |] eqn:R.
-      2: { simpl. trans False; [| set_solver].
-           apply neg_false. intros AL. inversion AL. subst.
-           congruence. }
-      split.
-      - intros AL. inversion AL. subst.
-        rewrite R in LOCK. inversion LOCK. subst. repeat split; eauto.
-        by intros [??].
-      - intros ([=]&[?[=]]&?). subst. econstructor.
-        rewrite R. repeat f_equal.
-        destruct x; [| done]. edestruct H6; eauto.
-    Qed.
-
-    Lemma allows_lock_impl_spec ρ st
-                                :
-      forall st', allows_lock ρ st st' <-> 
-              (allow_lock_impl ρ st = st' /\ (can_lock_st ρ st /\ ¬ active_st ρ st)).
-    Proof.
-      destruct st as [o t rm]. intros [o' t' rm'].
-      rewrite /allow_lock_impl /can_lock_st /active_st. simpl.  
-      destruct (rm !! ρ) as [[s e] |] eqn:R.
-      2: { simpl. trans False; [| set_solver].
-           apply neg_false. intros AL. inversion AL. subst.
-           congruence. }
-      split.
-      - intros AL. inversion AL. subst.
-        rewrite R in LOCK. inversion LOCK. subst. repeat split; eauto.
-        by intros [??].
-      - intros ([=]&[?[=]]&?). subst. econstructor.
-        rewrite R. repeat f_equal.
-        destruct x; [| done]. edestruct H6; eauto.
-    Qed. 
-      
-    Instance allows_lock_ex_dec:
-      forall st ρ, Decision (∃ st', allows_lock ρ st st'). 
-    Proof using.
-      intros [o t rm] ρ.
-      destruct (decide (rm !! ρ = Some (tl_L, false))).
-      - left. eexists. econstructor; eauto.
-      - right. intros [st' L]. inversion L. congruence. 
-    Defined.
-
-    Instance allows_unlock_ex_dec: 
-      forall st ρ, Decision (∃ st', allows_unlock ρ st st'). 
-    Proof using. 
-      intros [o t rm] ρ. 
-      (* destruct (role_of_dec rm (tl_U o, false)) as [[r LOCK] | FREE]. *)      
-      destruct (decide (rm !! ρ = Some (tl_U o, false))). 
-      - left. eexists. econstructor. eauto.
-      - right. intros [st' TRANS]. inversion TRANS. subst.
-        set_solver.
-    Defined. 
-
-    Definition tl_active_exts st: gset fl_EI := 
-      (* (if (allows_unlock_ex_dec st) then {[ flU ]} else ∅) ∪ *)
-      set_map (flU (M := tl_fair_model)) 
-          (filter (fun ρ => exists st', allows_unlock ρ st st') (dom (role_map st)))
-      ∪
-      set_map (flL (M := tl_fair_model)) 
-          (filter (fun ρ => exists st', allows_lock ρ st st') (dom (role_map st))).
-    
-    Lemma tl_active_exts_spec st ι:
-      ι ∈ tl_active_exts st <-> ∃ st', @fl_ETs tl_fair_model allows_unlock allows_lock ι st st'.
-    Proof using. 
-      unfold tl_active_exts.
-      rewrite elem_of_union.
-      rewrite !elem_of_map. repeat setoid_rewrite elem_of_filter.
-      erewrite exist_proper.
-      2: { intros. rewrite and_assoc. apply iff_and_impl_helper.
-           intros [? [? [?]]]. by apply elem_of_dom. }
-      rewrite or_comm. 
-      erewrite exist_proper.
-      2: { intros. rewrite and_assoc. apply iff_and_impl_helper.
-           intros [? [? [?]]]. by apply elem_of_dom. }
-      destruct ι; set_solver. 
-    Qed. 
-
-    Global Instance tl_FLE: FairLockExt tl_fair_model.
-    (* refine {| fl_active_exts := tl_active_exts |}.  *)
-    esplit.
-    apply tl_active_exts_spec.
-    Defined. 
-    
-    Instance ExtTL: ExtModel tl_fair_model := 
-      FL_EM tl_FLE. 
-    
   End TlExtTrans.
  
   Section ProgressProperties.
 
     Let ExtTL_FM := @ext_model_FM _ ExtTL. 
-
-    Lemma tl_init_st_wf n:
-      tl_state_wf (tl_init_st n). 
-    Proof using. 
-      rewrite /tl_init_st. 
-      red. split; [lia| ]. split; [| split]. 
-      - split; [lia| ]. intros [ρ [? RMρ]].
-        apply lookup_gset_to_gmap_Some in RMρ as [_ ?]. congruence.
-      - intros. rewrite lookup_gset_to_gmap_Some in H.
-        by destruct H. 
-      - intros. rewrite lookup_gset_to_gmap_Some in R1. 
-        by destruct R1.
-    Qed. 
 
     Section ProgressPropertiesImpl.
 
@@ -328,8 +592,8 @@ Section Model.
       Hypothesis (VALID: mtrace_valid tr).
       (* Hypothesis (FROM_INIT: forall st (INIT: tr S!! 0 = Some st), *)
       (*             exists n, st = tl_init_st n).  *)
-      Hypothesis (FROM_INIT: forall st (INIT: tr S!! 0 = Some st),
-                     tl_state_wf st). 
+      (* Hypothesis (FROM_INIT: forall st (INIT: tr S!! 0 = Some st), *)
+      (*                tl_state_wf st).  *)
       Hypothesis (FAIR: set_fair_model_trace (fun (ρ: fmrole ExtTL_FM) => 
                                                 exists r, ρ = inl r) tr).
 
@@ -343,14 +607,17 @@ Section Model.
           (fun st => role_map st !! ρ = Some (tl_L, true)) (other_step $ inl ρ).
       Proof using. 
         red. intros.
+        destruct st as [o1 t1 rm1 wf1], st' as [o2 t2 rm2 wf2]. simpl in *. 
         inversion STEP; subst.
         - assert (ρ0 ≠ ρ) as NEQ by (by intros ->). 
           inversion STEP0; subst; simpl in *; auto. 
           all: try by rewrite lookup_insert_ne; auto.
           subst st''. rewrite /advance_next. 
           destruct (role_of_dec _ _); simpl.
-          2: { rewrite lookup_insert_ne; auto. }
+          2: { inversion H4. subst. 
+               rewrite lookup_insert_ne; auto. }
           destruct s; simpl.
+          inversion H4. subst. 
           rewrite lookup_insert_ne.
           { rewrite lookup_insert_ne; auto. }
           intros ->. subst st'0 st'1. simpl in *. 
@@ -362,19 +629,21 @@ Section Model.
       Qed.
       
       Lemma advance_next_owner st:
-        owner (advance_next st ) = owner st.
-      Proof using. 
+        fst $ fst (advance_next st ) = fst $ fst st.
+      Proof using.
+        destruct st as [[]]. 
         rewrite /advance_next. destruct role_of_dec as [[? ?] | ?]; auto.
       Qed. 
             
       Lemma advance_next_ticket st:
-        ticket (advance_next st ) = ticket st.
+        snd $ fst (advance_next st ) = snd $ fst st.
       Proof using. 
+        destruct st as [[]]. 
         rewrite /advance_next. destruct role_of_dec as [[? ?] | ?]; auto.
       Qed.
 
       Lemma advance_next_helper_L o t (rm: tl_role_map) ρo ρ:
-        role_map (advance_next (<{o + 1, t, <[ρo := (tl_L, false)]> rm}>)) !! ρ = Some (tl_L, false) <-> (rm !! ρ = Some (tl_L, false) \/ ρ = ρo).
+        snd (advance_next (<{o + 1, t, <[ρo := (tl_L, false)]> rm}>)) !! ρ = Some (tl_L, false) <-> (rm !! ρ = Some (tl_L, false) \/ ρ = ρo).
       Proof using.
         (* clear eventual_release.  *)
         rewrite /advance_next.
@@ -396,256 +665,21 @@ Section Model.
           intros [? | ?]; done.
       Qed. 
 
-      Lemma advance_next_helper_U o t (rm: tl_role_map) ρo ρ k b
-        (RMρo: rm !! ρo = Some (tl_U o, true))
-        (UNIQ: forall ρ1 ρ2 k e1 e2 (R1: rm !! ρ1 = Some (tl_U k, e1))
-                 (R2: rm !! ρ2 = Some (tl_U k, e2)), ρ1 = ρ2)
-        (TKo: forall ρ k, rm !! ρ = Some (tl_U k, false) -> k = o):
-        role_map (advance_next (<{o + 1, t, <[ρo := (tl_L, false)]> rm}>)) !! ρ = Some (tl_U k, b) <-> (exists b', rm !! ρ = Some (tl_U k, b') /\ 
-                    (k = o + 1 /\ b = false /\ b' = true \/
-                     k ≠ o /\ k ≠ (o + 1) /\ b' = b)). 
-      Proof using.
-        rewrite /advance_next.
-        destruct role_of_dec as [[? ?] | ?]; simpl in *.
-        - assert (x ≠ ρo) as NEQ.
-          { intros ->. rewrite lookup_insert in e. congruence. }
-          rewrite lookup_insert_ne in e; auto.
-          destruct (decide (x = ρ)) as [-> | NEQ'].
-          { rewrite lookup_insert. split.
-            - intros. inversion H. eexists. eauto.
-            - intros [b' [RMρ ST]].
-              rewrite e in RMρ. intuition; congruence. }
-          rewrite lookup_insert_ne; auto.
-          destruct (decide (ρo = ρ)) as [-> | NEQ''].
-          { rewrite lookup_insert. rewrite RMρo. split; intros ST. 
-            - congruence.
-            - destruct ST as [b' ST]; intuition; subst.
-              + inversion H. lia.
-              + congruence. }
-          rewrite lookup_insert_ne; auto. split; intros; intuition. 
-          + exists b. split; auto. right. repeat split; auto; intros ->.
-            * destruct NEQ''. eapply UNIQ; eauto.
-            * destruct NEQ'. eapply UNIQ; eauto.
-          + destruct H as [b' [X ?]]. rewrite X.
-            repeat f_equal. intuition. subst.  
-            destruct NEQ'. eapply UNIQ; eauto. 
-        - destruct (decide (ρo = ρ)) as [-> | NEQ''].
-          { rewrite /advance_next. rewrite lookup_insert.
-            rewrite RMρo. split; intros; intuition; try congruence.
-            destruct H as [? [? [?|?]]]; subst.
-            - inversion H. lia.
-            - intuition. congruence. }
-          rewrite lookup_insert_ne; auto. split; intros; intuition; auto.
-          + exists b. split; auto. right. repeat split; auto. 
-            * intros ->. destruct NEQ''; eapply UNIQ; eauto.
-            * intros ->. destruct b.
-              ** destruct (n ρ). rewrite lookup_insert_ne; auto.
-              ** apply TKo in H. lia.
-          + destruct H as [? [? ?]]; intuition; subst; auto.
-            destruct (n ρ). rewrite lookup_insert_ne; auto.
-      Qed. 
-
-
-      Ltac simpl_li_eq := match goal with
-                          | H: <[?x:=?y]> ?m !! ?x = ?r |- _
-                            => rewrite lookup_insert in H
-                          end.
-      Ltac simpl_li_eq' := match goal with
-                           | |- <[?x:=?y]> ?m !! ?x = ?r
-                             => rewrite lookup_insert
-                           end.
-      
-      Ltac simpl_li_neq := match goal with
-                           | H: <[?x:=?y]> ?m !! ?x' = ?r, NE: ?x ≠ ?x' |- _ => 
-                               rewrite lookup_insert_ne in H; [| by apply NE]
-                           | H: <[?x:=?y]> ?m !! ?x' = ?r, NE: ?x' ≠ ?x |- _ =>
-                               rewrite lookup_insert_ne in H;
-                               [| by apply not_eq_sym; apply NE]
-                           end.
-      Ltac simpl_li_neq' := match goal with
-                           | NE: ?x ≠ ?x' |- <[?x:=?y]> ?m !! ?x' = ?r => 
-                               rewrite lookup_insert_ne; [| by apply NE]
-                           | NE: ?x' ≠ ?x |- <[?x:=?y]> ?m !! ?x' = ?r => 
-                               rewrite lookup_insert_ne;
-                               [| by apply not_eq_sym; apply NE]
-                           end.
-      
-      Ltac simpl_li := (repeat simpl_li_eq); (repeat simpl_li_neq);
-                       (try simpl_li_eq'); (try simpl_li_neq'). 
-
-      Lemma step_preserves_tl_state_wf st ℓ st'
-        (WF: tl_state_wf st) (STEP: fmtrans ExtTL_FM st ℓ st'):
-        tl_state_wf st'.
-      Proof using. 
-        destruct st as [o t rm]. destruct st' as [o' t' rm'].
-        red in WF. destruct WF as (LE & TKS & TKo & UNIQ).
-        inversion STEP; subst.
-        - inversion STEP0; subst; simpl in *; auto.
-          + rename o' into o.
-            split; [lia| ]. 
-            split; [| split]. 
-            * intros. specialize (TKS k).
-              destruct (decide (k = t)) as [-> | NEQ].
-              { split; [| lia]. intros T.
-                exists ρ. eexists. rewrite lookup_insert. split; eauto. }
-              etransitivity.
-              { etransitivity; [| apply TKS]. lia. }
-              split; intros; intuition. 
-              ** destruct H as (?&?&?). 
-                 do 2 eexists. rewrite lookup_insert_ne; eauto.
-                 intros <-. congruence.
-              ** destruct H as (?&?&?).
-                 do 2 eexists.
-                 rewrite <- H. symmetry. apply lookup_insert_ne.
-                 intros <-. rewrite lookup_insert in H. congruence.
-            * intros.
-              destruct (decide (ρ0 = ρ)) as [-> | NEQ].
-              2: { rewrite lookup_insert_ne in H; eauto. } 
-              rewrite lookup_insert in H. inversion H.
-              subst k next_en0.
-              destruct (decide (o = t)); congruence.
-            * intros. destruct (decide (ρ1 = ρ)), (decide (ρ2 = ρ)).
-              all: subst; simpl_li; inversion R1; inversion R2; subst; auto. 
-              1, 2: enough (k < k); [lia| ]; apply TKS; by eauto.
-              eapply UNIQ; eauto.
-          + subst st'' st'3 st'2 st'0 st' st'1.
-             assert (o' = o + 1 /\ t' = t) as [-> ->].
-             { rewrite /advance_next in H4.
-               destruct (role_of_dec _ _) as [[? ?] | ?]; by inversion H4. }
-             apply Nat.le_lteq in LE as [LT | ->].
-             2: { enough (t < t); [lia| ]. apply TKS. eauto. }
-             rewrite H4. red.
-             split; [lia| ]. split; [| split]. 
-             * intros. 
-               rewrite /advance_next in H4.
-               destruct (role_of_dec) as [[? ?] | ?]; simpl in *;
-                 inversion H4; subst rm'; clear H4.
-               ** destruct (decide (ρ = x)).
-                  { subst x. rewrite lookup_insert in e. congruence. }
-                  rewrite lookup_insert_ne in e; auto.
-                  destruct (decide (k = o)) as [-> | NEQ].
-                  { split; [lia| ]. intros (ρ' & e' & RMρ'). 
-                    destruct (decide (ρ' = ρ)).
-                    { subst ρ'. rewrite lookup_insert_ne in RMρ'; auto.
-                      rewrite lookup_insert in RMρ'. congruence. }
-                    destruct (decide (x = ρ')).
-                    { subst x. rewrite lookup_insert in RMρ'.
-                      inversion RMρ'. lia. }
-                    rewrite !lookup_insert_ne in RMρ'; auto.
-                    destruct n0. eapply UNIQ; eauto. }
-                  etransitivity; [etransitivity| ]; [| by apply (TKS k) |].
-                  { lia. }
-                  split.
-                  *** intros. destruct H as (?&?&?). 
-                      destruct (decide (k = o + 1)).
-                      **** subst. exists x, false. by rewrite lookup_insert.
-                      **** do 2 eexists. 
-                           rewrite !lookup_insert_ne; [by apply H| ..].
-                           { congruence. }
-                           intros <-. rewrite e in H. congruence.
-                  *** intros. destruct H as (?&?&?). 
-                      destruct (decide (k = o + 1)).
-                      **** subst. eauto.
-                      **** destruct (decide (x = x0)).
-                           all: subst; simpl_li; inversion H; subst.
-                           { lia. }
-                           destruct (decide (ρ = x0)). 
-                           all: subst; simpl_li; inversion H; subst; eauto. 
-               ** specialize (TKS k). 
-                  split.
-                  *** intros [GEk LTk].
-                      apply proj1 in TKS.
-                      specialize_full TKS; [lia| ]. destruct TKS as (?&?&TKS). 
-                      do 2 eexists. rewrite lookup_insert_ne; eauto.
-                      intros <-. rewrite R in TKS.
-                      inversion TKS. lia.
-                  *** intros. destruct H as (?&?&H). 
-                      destruct (decide (ρ = x)) as [-> | ?].
-                      { rewrite lookup_insert in H. congruence. }
-                      destruct (decide (k = o)) as [-> | NEQko].
-                      **** rewrite lookup_insert_ne in H; auto. 
-                           destruct n0. eapply UNIQ; eauto. 
-                      **** enough (o <= k < t); [lia| ]. apply TKS.
-                           rewrite lookup_insert_ne in H; eauto.
-             * intros. rewrite /advance_next in H4.
-               destruct role_of_dec as [[? ?] | ?]; simpl in *; 
-                 inversion H4; subst rm'; clear H4.
-               ** destruct (decide (ρ0 = x)), (decide (x = ρ)), (decide (ρ0 = ρ)); 
-                    do 2 (subst; simpl_li; inversion H; inversion e; subst; auto).
-                  apply TKo in H. subst k.
-                  destruct n1. eapply UNIQ; eauto. 
-               ** destruct (decide (ρ0 = ρ));
-                    subst; simpl_li; inversion H; subst; auto. 
-                  apply TKo in H. subst k.
-                  destruct n0. eapply UNIQ; eauto. 
-             * intros.
-               pose proof H4 as rm'_eq. apply (f_equal role_map) in rm'_eq. simpl in rm'_eq.
-               rewrite -rm'_eq in R1 R2. 
-               eapply advance_next_helper_U in R1, R2; auto.
-               destruct R1 as (?&?&R0), R2 as (?&?&R3).
-               destruct R0, R3; intuition; subst.
-               all: lia || eapply UNIQ; eauto.
-        - destruct ι; simpl in REL; inversion REL; subst o0 t0 rm0 o' t' rm'.
-          + split; auto. split; [| split]. 
-            * intros. etransitivity; [etransitivity|]; [| apply TKS |]; [reflexivity|..].
-              split; intros; intuition; destruct H as (?&?&?). 
-              ** destruct (decide (x = ρ)) as [-> | NEQ].
-                 *** exists ρ, true. rewrite lookup_insert. congruence.
-                 *** exists x, x0. rewrite lookup_insert_ne; auto.
-              ** destruct (decide (x = ρ)) as [-> | NEQ].
-                 *** rewrite lookup_insert in H.
-                     exists ρ, false. congruence.
-                 *** rewrite lookup_insert_ne in H; auto.
-                     eauto.
-            * intros. eapply TKo; eauto. rewrite -H.
-              symmetry. apply lookup_insert_ne.
-              intros ->. rewrite lookup_insert in H. congruence.
-            * intros.
-              destruct (decide (ρ1 = ρ)), (decide (ρ2 = ρ)).
-              all: subst; simpl_li; inversion R1; inversion R2; subst; auto. 
-              all: eapply UNIQ; eauto.
-          + split; auto. split; [| split]. 
-            * intros. etransitivity; [etransitivity|]; [| apply TKS |]; [reflexivity|..].
-              split; intros; intuition; destruct H as (?&?&?). 
-              ** exists x, x0. destruct (decide (x = ρ)); 
-                   subst; simpl_li; [congruence| auto]. 
-              ** destruct (decide (x = ρ)); subst; simpl_li; inversion H; eauto.
-            * intros. destruct (decide (ρ0 = ρ)); subst; simpl_li; try congruence.
-              eapply TKo; eauto.
-            * intros.
-              destruct (decide (ρ1 = ρ)), (decide (ρ2 = ρ)).
-              all: subst; simpl_li; inversion R1; inversion R2; subst; auto. 
-              all: eapply UNIQ; eauto.
-      Qed.
-
-
-      Lemma tl_valid_trace_states i st (ITH: tr S!! i = Some st):
-        tl_state_wf st. 
-      Proof using FROM_INIT VALID.
-        gd st. induction i.
-        { intros. by apply FROM_INIT. }
-
-        pose proof (trace_has_len tr) as [len LEN]. 
-        intros [rm' t' o']. rewrite -Nat.add_1_r. intros ITH'.
-        forward eapply trace_lookup_dom_strong with (i := i) as [_ ITH]; eauto.
-        specialize_full ITH; [eapply state_lookup_dom; eauto| ].
-        destruct ITH as (?&?&?&ITH). 
-        forward eapply trace_valid_steps' as STEP; eauto.
-        apply state_label_lookup in ITH.
-        destruct ITH as (?&ITH0&?). 
-        rewrite ITH' in ITH0. inversion ITH0. subst.
-        eapply step_preserves_tl_state_wf; eauto.
-      Qed.
-
       Lemma step_counters_mono st ℓ st' (STEP: fmtrans ExtTL_FM st ℓ st'):
         owner st <= owner st' /\ ticket st <= ticket st'.
       Proof using.
+        destruct st as [o1 t1 rm1 wf1], st' as [o2 t2 rm2 wf2].
         inversion STEP; subst.
-        - inversion STEP0; subst; simpl in *; try lia.
-          subst st'1 st'0 st''. simpl in *.
-          rewrite advance_next_owner advance_next_ticket. simpl. lia.
+        - inversion STEP0; subst. 
+          all: try by (simpl in *; lia).
+          subst st'1 st'0 st''.
+          pose proof (@f_equal _ _ (fst ∘ fst) _ _ H4) as O.
+          unfold compose in O. rewrite advance_next_owner in O. 
+          pose proof (@f_equal _ _ (snd ∘ fst) _ _ H4) as T.
+          unfold compose in T. rewrite advance_next_ticket in T. 
+          simpl in *. lia. 
         - destruct ι; simpl in REL; inversion REL; subst; simpl; lia.
-      Qed. 
+      Qed.
 
       Lemma trace_counters_mono i j st st'
         (ITH: tr S!! i = Some st) (JTH: tr S!! j = Some st') (LE: i <= j):
@@ -685,25 +719,25 @@ Section Model.
         (OTHER: proj_role (inr $ env ι) ≠ ρ):
           role_map st2 !! ρ = role_map st1 !! ρ.
       Proof.
+        destruct st1 as [o1 t1 rm1 wf1], st2 as [o2 t2 rm2 wf2].
         destruct ι; inversion STEP; subst; simpl in *.
         all: by apply lookup_insert_ne.
       Qed. 
 
       Lemma has_lock_kept_others (ρ: tl_role) b:
         @label_kept_state ExtTL_FM 
-          (fun st => tl_state_wf st /\ role_map st !! ρ = Some (tl_U (owner st), b)
-          ) (other_proj ρ).
+          (fun st => role_map st !! ρ = Some (tl_U (owner st), b)) (other_proj ρ).
       Proof using. 
-        red. intros. destruct Pst as (WF & OWNER).
-        split. 
-        { eapply step_preserves_tl_state_wf; eauto. }
+        red. intros. 
+        destruct st as [o1 t1 rm1 wf1], st' as [o2 t2 rm2 wf2].
+        rename Pst into OWNER.
         inversion STEP; subst.
         - rewrite /has_lock_st. assert (ρ0 ≠ ρ) as NEQ by (by intros ->). 
           inversion STEP0; subst; simpl in *; eauto. 
           { rewrite lookup_insert_ne; eauto. }
-          destruct NEQ. eapply WF; eauto.
+          destruct NEQ. eapply wf1; eauto. 
         - destruct ι; simpl in REL; inversion REL; subst; simpl in *.
-          + assert (ρ0 = ρ) as -> by (eapply WF; eauto).
+          + assert (ρ0 = ρ) as -> by (eapply wf1; eauto).
             inversion STEP. subst.
             eapply ext_trans_others_kept in REL0; eauto. congruence. 
           + rewrite lookup_insert_ne; eauto.
@@ -711,19 +745,19 @@ Section Model.
       
       Lemma has_lock_kept (ρ: tl_role) (o: nat):
         @label_kept_state ExtTL_FM 
-          (fun st => tl_state_wf st /\ owner st = o /\ has_lock_st ρ st) (other_step $ inl ρ).
-      Proof using FROM_INIT.
-        red. intros. destruct Pst as (WF & OW & [b OWNER]).
-        split. 
-        { eapply step_preserves_tl_state_wf; eauto. }
+          (fun st => owner st = o /\ has_lock_st ρ st) (other_step $ inl ρ).
+      Proof using.
+        red. intros. 
+        destruct st as [o1 t1 rm1 wf1], st' as [o2 t2 rm2 wf2].
+        destruct Pst as (WF & OW & OWNER).
         inversion STEP; subst.
         - rewrite /has_lock_st. assert (ρ0 ≠ ρ) as NEQ by (by intros ->). 
           inversion STEP0; subst; simpl in *; eauto. 
           { split; auto. rewrite lookup_insert_ne; eauto. }
-          destruct NEQ. eapply WF; eauto.
+          destruct NEQ. eapply wf1; eauto.
         - destruct ι; simpl in REL; inversion REL; subst; simpl in *.
           all: split; [auto| red]. 
-          + assert (ρ0 = ρ) as -> by (eapply WF; eauto).
+          + assert (ρ0 = ρ) as -> by (eapply wf1; eauto).
             rewrite lookup_insert. eauto.
           + rewrite lookup_insert_ne; eauto.
             intros ->. congruence.
@@ -732,20 +766,19 @@ Section Model.
       (* it turns out shorter to just repeat the previous proof *)
       Lemma has_lock_en_kept (ρ: tl_role) (o: nat):
         @label_kept_state ExtTL_FM 
-          (fun st => tl_state_wf st /\ owner st = o /\
-                    role_map st !! ρ = Some (tl_U o, true)) (other_step $ inl ρ).
-      Proof using FROM_INIT.
-        red. intros. destruct Pst as (WF & OW & OWNER).
-        split. 
-        { eapply step_preserves_tl_state_wf; eauto. }
+          (fun st => owner st = o /\ role_map st !! ρ = Some (tl_U o, true)) (other_step $ inl ρ).
+      Proof using. 
+        red. intros. 
+        destruct st as [o1 t1 rm1 wf1], st' as [o2 t2 rm2 wf2].        
+        destruct Pst as (OW & OWNER).
         inversion STEP; subst.
         - rewrite /has_lock_st. assert (ρ0 ≠ ρ) as NEQ by (by intros ->). 
           inversion STEP0; subst; simpl in *; eauto. 
           { split; auto. rewrite lookup_insert_ne; eauto. }
-          destruct NEQ. eapply WF; eauto.
+          destruct NEQ. eapply wf1; eauto.
         - destruct ι; simpl in REL; inversion REL; subst; simpl in *.
           all: split; [auto| ]. 
-          + assert (ρ0 = ρ) as -> by (eapply WF; eauto).
+          + assert (ρ0 = ρ) as -> by (eapply wf1; eauto).
             rewrite lookup_insert. eauto.
           + rewrite lookup_insert_ne; eauto.
             intros ->. congruence.
@@ -754,20 +787,19 @@ Section Model.
       (* it turns out shorter to just repeat the previous proof *)
       Lemma has_lock_active_kept (ρ: tl_role) (o: nat):
         @label_kept_state ExtTL_FM 
-          (fun st => tl_state_wf st /\ owner st = o /\
-                    role_map st !! ρ = Some (tl_U o, true)) (other_step $ inl ρ).
-      Proof using FROM_INIT.
-        red. intros. destruct Pst as (WF & OW & OWNER).
-        split. 
-        { eapply step_preserves_tl_state_wf; eauto. }
+          (fun st => owner st = o /\ role_map st !! ρ = Some (tl_U o, true)) (other_step $ inl ρ).
+      Proof using. 
+        red. intros. 
+        destruct st as [o1 t1 rm1 wf1], st' as [o2 t2 rm2 wf2].        
+        destruct Pst as (OW & OWNER).
         inversion STEP; subst.
         - rewrite /has_lock_st. assert (ρ0 ≠ ρ) as NEQ by (by intros ->). 
           inversion STEP0; subst; simpl in *; eauto. 
           { split; auto. rewrite lookup_insert_ne; eauto. }
-          destruct NEQ. eapply WF; eauto.
+          destruct NEQ. eapply wf1; eauto.
         - destruct ι; simpl in REL; inversion REL; subst; simpl in *.
           all: split; [auto| ]. 
-          + assert (ρ0 = ρ) as -> by (eapply WF; eauto).
+          + assert (ρ0 = ρ) as -> by (eapply wf1; eauto).
             rewrite lookup_insert. eauto.
           + rewrite lookup_insert_ne; eauto.
             intros ->. congruence.
@@ -775,86 +807,99 @@ Section Model.
 
       Lemma lock_wait_kept (ρ ρo: tl_role) o n:
         @label_kept_state ExtTL_FM 
-          (fun st => exists b bo, tl_state_wf st /\ 
+          (fun st => exists b bo, 
                    role_map st !! ρ = Some (tl_U n, b) /\ 
                    role_map st !! ρo = Some (tl_U o, bo) /\
                    owner st = o) (other_step $ inl ρo).
-      Proof using FROM_INIT.
-        red. intros. destruct Pst as (b & bo & WF & TKn & OWNER & OWo).
-        forward eapply (has_lock_kept ρo (owner st) _ _ _ _ _ STEP). Unshelve.
+      Proof using.
+        red. intros.
+        destruct st as [o1 t1 rm1 wf1], st' as [o2 t2 rm2 wf2].        
+        destruct Pst as (b & bo & TKn & OWNER & OWo).
+        simpl in *. 
+        forward eapply (has_lock_kept ρo o1 _ _ _ _ _ STEP). Unshelve.
         3: { eauto. }
-        2: { repeat split; eauto. red. eauto. rewrite OWo. eauto. }
-        intros (WF' & OWNER' & LOCK'). 
-        
-        destruct (decide (ρo = ρ)) as [-> | NEQ].
-        { assert (n = owner st /\ bo = b) as [-> ->] by (split; congruence). 
-          red in LOCK'. destruct LOCK' as [e LOCK']. 
-          exists e, e. repeat split; eauto; congruence. }
+        2: { repeat split; eauto. red. eauto. simpl in *. rewrite OWo. eauto. }
+        intros (OWNER' & LOCK'). 
 
-        assert (owner st < n /\ b = true) as [LT ->].
-        { destruct st as [o_ t rm]. simpl in *. subst o_.  
-          destruct WF as (LE & TKS & TKO & UNIQ).
+        destruct (decide (ρo = ρ)) as [-> | NEQ].
+        { assert (n = o1 /\ bo = b) as [-> ->] by (split; congruence). 
+          red in LOCK'. destruct LOCK' as [e LOCK']. 
+          exists e, e. simpl in *. repeat split; eauto; congruence. }
+
+        assert (o1 < n /\ b = true) as [LT ->].
+        { 
+          destruct wf1 as (LE & TKS & TKO & UNIQ).
           destruct (decide (n = o)) as [-> | NEQ'].
           { destruct NEQ. eapply UNIQ; eauto. }
-          specialize (TKS n). apply proj2 in TKS. specialize_full TKS; [eauto|]. 
+          pose proof (TKS n) as TKS'. apply proj2 in TKS'. specialize_full TKS'; [eauto|]. 
           destruct b; [split; [lia|auto]| ].
-          by apply TKO in TKn. }
+          apply TKO in TKn. subst. done. }
 
         destruct LOCK' as [bo' LOCK'].
-        exists true, bo'. repeat split; eauto; try congruence.  
+        exists true, bo'.
+        simpl in *.
+        repeat split; eauto; try congruence.  
 
         inversion STEP; subst.
-        - inversion STEP0; subst; simpl in *.
-          + rewrite lookup_insert_ne; auto.
+        - inversion STEP0; subst.
+          + simpl in *. rewrite lookup_insert_ne; auto.
             intros ->. congruence.
-          + congruence.
+          + simpl in *. congruence.
           + subst st''.
-            rewrite advance_next_owner in OWNER'.  subst st'0. simpl in *. lia.
+            pose proof (advance_next_owner st') as O. rewrite H4 in O.
+            subst st'0. simpl in *. lia.
         - destruct ι; simpl in REL; inversion REL; subst; simpl in *. 
           all: rewrite lookup_insert_ne; eauto; intros ->; congruence.
       Qed.
 
       Lemma lock_wait_active_kept (ρ ρo: tl_role) o n:
         @label_kept_state ExtTL_FM 
-          (fun st => exists b, tl_state_wf st /\ 
+          (fun st => exists b, 
                    role_map st !! ρ = Some (tl_U n, b) /\ 
                    role_map st !! ρo = Some (tl_U o, true) /\
                    owner st = o) (other_step $ inl ρo).
-      Proof using FROM_INIT.
-        red. intros. destruct Pst as (b & WF & TKn & OWNER & OWo).
-        forward eapply (has_lock_active_kept ρo (owner st) _ _ _ _ _ STEP). Unshelve.
+      Proof using. 
+        red. intros.
+        destruct st as [o1 t1 rm1 wf1], st' as [o2 t2 rm2 wf2].        
+        destruct Pst as (b & TKn & OWNER & OWo).
+        forward eapply (has_lock_active_kept ρo o1 _ _ _ _ _ STEP). Unshelve.
         3: { eauto. }
-        2: { repeat split; eauto. rewrite OWo. eauto. }
-        intros (WF' & OWNER' & LOCK'). 
+        2: { simpl in *. repeat split; eauto. rewrite OWo. eauto. }
+        intros (OWNER' & LOCK'). 
         
         destruct (decide (ρo = ρ)) as [-> | NEQ].
-        { assert (n = owner st) as -> by congruence.
+        { simpl in *. assert (n = o1) as -> by congruence.
           exists true. repeat split; eauto; congruence. } 
 
-        assert (owner st < n /\ b = true) as [LT ->].
-        { destruct st as [o_ t rm]. simpl in *. subst o_.  
-          destruct WF as (LE & TKS & TKO & UNIQ).
+        assert (o1 < n /\ b = true) as [LT ->].
+        { 
+          destruct wf1 as (LE & TKS & TKO & UNIQ).
           destruct (decide (n = o)) as [-> | NEQ'].
           { destruct NEQ. eapply UNIQ; eauto. }
-          specialize (TKS n). apply proj2 in TKS. specialize_full TKS; [eauto|]. 
+          pose proof (TKS n) as TKS'. apply proj2 in TKS'. specialize_full TKS'; [eauto|].
+          simpl in *. 
           destruct b; [split; [lia|auto]| ].
-          by apply TKO in TKn. }
+          apply TKO in TKn. subst. lia. }
 
-        destruct LOCK' as [bo' LOCK'].
-        exists true. split; eauto; try congruence. apply and_assoc. split; [| congruence].
+        simpl in *. subst.
+        (* destruct LOCK' as [bo' LOCK']. *)
+        exists true. split; eauto; try congruence.
+        (* apply and_assoc. split; [| congruence]. *)
 
         inversion STEP; subst.
-        - inversion STEP0; subst; simpl in *.
-          + assert (ρ0 ≠ ρ) by congruence. 
+        - inversion STEP0.
+          + subst; simpl in *.
+            assert (ρ0 ≠ ρ) by congruence. 
             rewrite lookup_insert_ne; auto. 
-            split; auto. 
-            rewrite lookup_insert_ne; auto. 
-            intros ->. congruence.
-          + split; auto. 
+            (* split; auto.  *)
+            (* rewrite lookup_insert_ne; auto.  *)
+            (* intros ->. congruence. *)
+          + subst; simpl in *. done. 
           + subst st''.
-            rewrite advance_next_owner in OWNER'.  subst st'0. simpl in *. lia.
-        - destruct ι; simpl in REL; inversion REL; subst; simpl in *. 
-          all: split; auto; rewrite lookup_insert_ne; eauto; intros ->; congruence.
+            pose proof (advance_next_owner st') as O. rewrite H4 in O.
+            simpl in *. subst. lia.
+        - destruct ι; simpl in REL; inversion REL; subst; simpl in *.
+          all: rewrite lookup_insert_ne; eauto; intros ->; congruence.
       Qed.
 
       Definition is_unused ρ st :=
@@ -868,7 +913,6 @@ Section Model.
         - exact has_lock_st.
         - exact active_st.
         - exact is_unused. 
-        - exact tl_state_wf.
         (* ???  *)
         (* 1-4: solve_decision.  *)
         (* all: solve_decision. *)
@@ -881,16 +925,15 @@ Section Model.
       Let tl_eventual_release := @eventual_release _ tl_FLP ExtTL.  
 
       Lemma has_lock_unique st ρ1 ρ2
-        (WF: tl_state_wf st)
         (LOCK1: has_lock_st ρ1 st) (LOCK2: has_lock_st ρ2 st):
         ρ1 = ρ2.
       Proof using.
         destruct LOCK1 as [? L1]. destruct LOCK2 as [? L2].
-        destruct st. eapply WF; eauto.
+        eapply (tl_wf st); eauto.  
       Qed.
 
-      Lemma lock_eventually_acquired_iteration o t rm ρ i d
-        (ST: tr S!! i = Some <{ o, t, rm }>)
+      Lemma lock_eventually_acquired_iteration o t rm wf ρ i d
+        (ST: tr S!! i = Some (mkTlSt o t rm wf) )
         (R: rm !! ρ = Some (tl_U (S o + d), true))
         (EV_REL: tl_eventual_release tr ρ i):
         ∃ (n : nat) (st': tl_st),
@@ -899,16 +942,17 @@ Section Model.
           i < n ∧ tr S!! n = Some st' ∧ owner st' = o + 1 /\
           role_map st' !! ρ = Some (tl_U (S o + d), e') /\
           forall k st_k, i <= k < n + a → tr S!! k = Some st_k → ¬ has_lock_st ρ st_k.
-      Proof using VALID FROM_INIT FAIR.
-        assert (exists ρo, has_lock_st ρo <{ o, t, rm }>) as [ρo LOCK].
-        { apply tl_valid_trace_states in ST as (LE & TKS & _).
+      Proof using VALID FAIR.
+        assert (exists ρo, has_lock_st ρo (mkTlSt o t rm wf)) as [ρo LOCK].
+        {
+          (* apply tl_valid_trace_states in ST as (LE & TKS & _). *)
+          pose proof wf as (LE & TKS & ?).
           apply Lt.le_lt_or_eq_stt in LE as [LT | ->].
           2: { enough (S t + d < t); [lia| ]. apply TKS. eauto. }
           specialize (TKS o). apply proj1 in TKS. specialize_full TKS; auto. }
         assert (ρo ≠ ρ) as NEQ.
         { intros ->. red in LOCK. destruct LOCK as [? LOCK]. 
           rewrite R in LOCK. inversion LOCK. lia. }
-
         
         assert ( ∃ k : nat,
          ClassicalFacts.Minimal
@@ -916,7 +960,7 @@ Section Model.
               ∃ st'' : ext_model_FM,
                 tr S!! k0 = Some st'' ∧ i ≤ k0 ∧ active_st ρo st'') k
 ) as HH.
-        { destruct (decide (active_st ρo (<{ o, t, rm }>))).
+        { destruct (decide (active_st ρo (mkTlSt o t rm wf))).
           { exists i. split; eauto.
             intros ? (?&?&?). lia. }
         
@@ -937,8 +981,7 @@ Section Model.
         all: eauto.
         { eexists. split; [apply ST|]. 
           red in LOCK. destruct LOCK as [? LOCK]. do 2 eexists.
-          split; [| split]; [..|split]; eauto. 
-          eapply tl_valid_trace_states; eauto. }
+          split; [| split]; [..|split]; eauto. }
         { intros. destruct IKJ as [[v ->]%Nat.le_sum KJ].
           intros ->. enough (k <= i + v); [lia| ]. apply MINk.
           forward eapply (proj1 (label_lookup_states tr (i + v))) as HH; eauto.
@@ -949,7 +992,7 @@ Section Model.
           inversion STEP; subst.
           apply active_st_enabled.
           eapply fm_live_spec; eauto. }
-        simpl in LOCK'. destruct LOCK' as (b & bo & WF' & R' & Ro' & OW').
+        simpl in LOCK'. destruct LOCK' as (b & bo & R' & Ro' & OW').
         assert (bo = true) as ->.
         { red in ENρo. destruct ENρo. congruence. }
         
@@ -961,32 +1004,40 @@ Section Model.
           apply active_st_enabled. red.
           destruct Pst. eexists. apply H. }
         { simpl. repeat split; eauto. }
-        intros (j & st'' & [[LEkj STEPj] MINj] & JTH & b_ & WF'' & RMρ'' & RMρo'' & OW'').
+        intros (j & st'' & [[LEkj STEPj] MINj] & JTH & b_ & RMρ'' & RMρo'' & OW'').
+        pose proof (tl_wf st'') as WF''. 
         assert (b_ = true) as ->.
         { destruct b_; auto.
-          destruct st''; simpl in *. destruct WF'' as (? & ? & TKo'' & _).
+          pose proof (tl_wf st'') as (? & ? & TKo'' & _).
+          destruct st''; simpl in *.
           apply TKo'' in RMρ''. lia. }
 
         forward eapply (proj1 (label_lookup_states tr j)) as [_ [st''' J'TH]]; eauto.
         exists (j + 1), st'''. split; [lia| ]. split; [auto| ].
+        destruct st'', st'''. simpl in *.  
         forward eapply (trace_valid_steps' _ _ VALID j) as STEP; eauto.
         { eapply state_label_lookup; eauto. }
-        inversion STEP; subst. inversion STEP0; subst; simpl in *.
-        { congruence. }
-        { rewrite RMρo'' in R0. inversion R0. lia. }
-        subst st''0. split.
-        { rewrite advance_next_owner. subst st'0. simpl. lia. }
+        inversion STEP; subst. inversion STEP0; subst.
+        { simpl in *. congruence. }
+        { simpl in *. rewrite RMρo'' in R0. inversion R0. lia. }
+        pose proof (advance_next_owner st'0) as O. 
+        pose proof (advance_next_ticket st'0) as T.
+        (* pose proof (advance_next_helper_U st'0) as OU. *)
+        fold st'' in O, T. rewrite H4 in O, T. simpl in *. 
+        split.
+        { lia. }
 
-        assert (exists ρ', rm0 !! ρ' = Some (tl_U (S (owner st')), true)) as [ρ' RM'].
-        { destruct WF'' as (? & ? & ? & ?).          
-          pose proof (H0 (S o + d)) as B. apply proj2 in B. specialize_full B.
-          { rewrite OW''. eauto. }
-          pose proof (H0 (S o)) as RR. apply proj1 in RR. specialize_full RR.
+        assert (exists ρ', role_map0 !! ρ' = Some (tl_U (S (owner st')), true)) as [ρ' RM'].
+        {
+          destruct WF'' as (? & ? & ? & ?).
+          pose proof (H0 (S (owner st') + d)) as B. apply proj2 in B. specialize_full B.
+          { eauto. }
+          pose proof (H0 (S (owner st'))) as RR. apply proj1 in RR. specialize_full RR.
           { lia. }
           destruct RR as (ρ' & b' & R'_).
-          exists ρ'. rewrite <- OW''. destruct b'; auto.
+          exists ρ'. destruct b'; auto.
           apply H1 in R'_. lia. }
-        rewrite -OW'' -Nat.add_1_r in RM'.
+        rewrite -Nat.add_1_r in RM'.
         assert (ρo ≠ ρ') as NEQ'.
         { intros <-. rewrite RMρo'' in RM'. inversion RM'. lia. }
         subst st'0. simpl. rewrite /advance_next.
@@ -1001,23 +1052,23 @@ Section Model.
         
         assert (∀ k0 st_k, i <= k0 < j + 1 → tr S!! k0 = Some st_k → ¬ has_lock_st ρ st_k) as NOLOCKρ.
         { destruct st' as [o' t' rm']. simpl in *.
-          assert (o' = o) as -> by lia. 
+          (* assert (o' = o) as -> by lia. *)
           intros. intros LOCKρ'.
           forward eapply steps_keep_state with (i := i) (j := k0) (k := k0). 
           3: { apply has_lock_kept. }
           all: eauto. 
-          { eexists. repeat split; eauto using tl_valid_trace_states. }
+          (* { eexists. repeat split; eauto using tl_valid_trace_states. } *)
           { intros. intros ->.
             specialize (MINk k1). specialize_full MINk.
             { forward eapply (proj1 (label_lookup_states tr k1)) as [[? ?] [? ?]]; [eauto| ].
               eexists. split; eauto. split; [lia| ].
               apply active_st_enabled.
               red. enough (inl ρo ∈ live_roles ExtTL_FM x).
-              { simpl in H4. rewrite /ext_live_roles in H4.
-                apply elem_of_union in H4 as [? | ?].
-                - apply elem_of_map_inj_gset in H4; [auto | congruence].
-                - rewrite set_map_compose_gset in H4.
-                  apply elem_of_map_1 in H4 as (? & ? & ?). congruence. }
+              { simpl in H5. rewrite /ext_live_roles in H5.
+                apply elem_of_union in H5 as [? | ?].
+                - apply elem_of_map_inj_gset in H5; [auto | congruence].
+                - rewrite set_map_compose_gset in H5.
+                  apply elem_of_map_1 in H5 as (? & ? & ?). congruence. }
               eapply fm_live_spec; eauto.
               pose proof (trace_valid_steps'' _ _ VALID k1). 
               eapply (trace_valid_steps'' _ _ VALID k1); eauto. }
@@ -1025,39 +1076,40 @@ Section Model.
             move MINj at bottom. specialize (MINj k1 (conj MINk H1)).
             lia. }
           { lia. }
-          intros (? & ? & ?). 
+          intros (? & ?). 
           destruct NEQ'''. eapply has_lock_unique; eauto. }
 
+        subst st'' st'4 st'2. inversion H4. subst.  
         destruct (decide (ρ = ρ')) as [-> | ?].
-        { rewrite lookup_insert.
+        { subst. simpl in *.
+          rewrite lookup_insert.
           rewrite RMρ'' in e. inversion e. 
           destruct (decide (d = 0)) as [-> | ?]; [| lia]; auto.
           rewrite !Nat.add_0_r. auto. }
         do 2 (rewrite lookup_insert_ne; auto).
         destruct (decide (d = 0)) as [-> | ?]; split; try rewrite !Nat.add_0_r; auto.
-        { rewrite Nat.add_0_r -Nat.add_1_r -OW'' in RMρ''.
+        { rewrite Nat.add_0_r -Nat.add_1_r in RMρ''.
           destruct n. eapply WF''; eauto. }
         intros. destruct (decide (k0 = j + 1)) as [? | ?].
         2: { eapply NOLOCKρ; eauto. lia. }
-        subst. rewrite J'TH in H0. inversion H0. subst st_k. clear H0.
-        rewrite /has_lock_st advance_next_owner /=.
-        intros [e' LOCK']. apply advance_next_helper_U in LOCK'; eauto.
-        2, 3: by apply WF''.
-        destruct LOCK' as [e'' [RM0ρ bar]].
-        rewrite RMρ'' in RM0ρ. inversion RM0ρ. lia.
+        subst. rewrite J'TH in H2. inversion H2. subst st_k. clear H2.
+        rewrite /has_lock_st. 
+        intros [e' LOCK'].  simpl in LOCK'. 
+        do 2 (rewrite lookup_insert_ne in LOCK'; [| done]). 
+        rewrite RMρ'' in LOCK'. inversion LOCK'. lia.
       Qed.
         
-      Lemma lock_eventually_acquired o t rm ρ i wt 
-        (ST: tr S!! i = Some <{ o, t, rm }>)
+      Lemma lock_eventually_acquired o t rm wf ρ i wt 
+        (ST: tr S!! i = Some (mkTlSt o t rm wf))
         (WAIT: o ≠ wt)
         (R: rm !! ρ = Some (tl_U wt, true))
         (EV_REL: tl_eventual_release tr ρ i):
         ∃ (n : nat) (st' : tl_st),
           i < n ∧ tr S!! n = Some st' ∧ has_lock_st ρ st' ∧ ¬ active_st ρ st'.
-      Proof using VALID FROM_INIT FAIR.
+      Proof using VALID FAIR.
         assert (o < wt) as LT.
-        { apply PeanoNat.Nat.le_neq. split; auto. 
-          apply tl_valid_trace_states in ST. apply ST. eauto. }
+        { apply PeanoNat.Nat.le_neq. split; auto.
+          apply wf. eauto. }
         apply Nat.le_succ_l in LT. apply Nat.le_sum in LT as [d ->]. clear WAIT.
         gd i. gd o. gd rm. gd t. induction d.
         { intros. eapply lock_eventually_acquired_iteration in ST; eauto.
@@ -1076,10 +1128,11 @@ Section Model.
         simpl in ST. destruct ST as (n&st'&ST). 
         destruct st'. simpl in *.
         replace (S (o + S d)) with (S (S o) + d) in ST by lia.
-        rewrite decide_False in ST; [| lia].
-        destruct ST as (ST&ST0&ST1&ST2&ST3). 
-        eapply IHd in ST2.
-        2: { rewrite -Nat.add_1_r -ST1. eauto. }
+        rewrite decide_False in ST; [| lia].        
+        destruct ST as (ST&ST0&ST1&ST2&ST3).
+        rewrite ST1 Nat.add_1_r in tl_wf0, ST0. 
+        eapply IHd with (i := n) in ST2. 
+        2: { apply ST0. }
         2: { do 2 red. intros. subst. simpl in *.
              rename ST3 into NOLOCKρ.
              do 2 red in EV_REL.
@@ -1142,7 +1195,7 @@ Section Model.
         (EV_REL: tl_eventual_release tr ρ i):
         exists n st', i < n /\ tr S!! n = Some st' /\ has_lock_st ρ st' /\
                    ¬ role_enabled_model (ρ: fmrole tl_fair_model) st'.
-      Proof using VALID FAIR FROM_INIT.
+      Proof using VALID FAIR.
         red in CAN_LOCK. destruct CAN_LOCK as [e RMρ].
         assert (e = true) as -> by (destruct ACT; congruence). 
 
@@ -1165,9 +1218,10 @@ Section Model.
         { by eapply state_label_lookup. }
           
         simpl in TRANS. inversion TRANS as [? ? ? TRANS'| ]; subst.
-        inversion TRANS'; subst; simpl in *.
-        all: try by rewrite RMρ' in R.
-        destruct (decide (o = t)) as [<- | WAIT]. 
+        destruct st' as [o1 t1 rm1 wf1], st'' as [o2 t2 rm2 wf2]. 
+        inversion TRANS'; subst.
+        all: try by (simpl in *; rewrite RMρ' in R). 
+        destruct (decide (o2 = t1)) as [<- | WAIT]. 
         { exists (i + d + 1). eexists.
           repeat split; [lia|..]; try by eauto.
           - red. eexists. simpl. rewrite lookup_insert. eauto. 
@@ -1201,17 +1255,25 @@ Section Model.
       (fun _ => True).
     Proof.
       simpl. rewrite /is_unused. 
-      red. intros. pose proof Pst as Pst'%not_elem_of_dom. 
+      red. intros.
+      destruct st as [o1 t1 rm1 wf1], st' as [o2 t2 rm2 wf2]. 
+      pose proof Pst as Pst'%not_elem_of_dom. 
       inversion STEP; subst.
-      + inversion STEP0; subst; simpl in *; auto; try set_solver.
+      + inversion STEP0; subst; auto; try set_solver.
         { rewrite dom_insert. apply not_elem_of_union. split; auto.
           apply not_elem_of_singleton_2. intros <-.
           by rewrite Pst' in R. }
-        subst st'' st'0. simpl. rewrite /advance_next. simpl.
+
+        (* fold st''.  *)
+        enough (ρ ∉ dom $ snd st'').
+        { rewrite H4 in H. simpl in *. congruence. } 
+        
+        subst st'' st'0. rewrite /advance_next. simpl.
         assert (ρ ≠ ρ0) as NEQ'.
         { intros <-. by rewrite Pst' in R. }
         destruct role_of_dec as [[r ?]| ].
         2: { set_solver. }
+        
         simpl. rewrite !dom_insert.
         apply not_elem_of_union. split; [| set_solver].
         apply not_elem_of_singleton_2. intros <-.
@@ -1227,7 +1289,68 @@ Section Model.
           by rewrite Pst' in LOCK.
     Qed.
     
+    Definition allow_unlock_impl (ρ: fmrole tl_fair_model) (st: tl_st): tl_st.
+      destruct st as [o t rm wf].
+      destruct (decide (rm !! ρ = Some (tl_U o, false))) as [R|]. 
+      2: { exact (mkTlSt o t rm wf). }
+      pose proof (allows_unlock_step ρ o t rm R).
+      pose proof (allows_unlock'_preserves_tl_state_wf _ _ _ H wf).
+      esplit. apply H0. 
+    Defined. 
+      
+    Lemma allows_unlock_impl_spec ρ st:
+      forall st', allows_unlock ρ st st' <-> 
+              (allow_unlock_impl ρ st = st' /\ (has_lock_st ρ st /\ ¬ active_st ρ st)).
+    Proof.
+      destruct st as [o t rm]. intros [o' t' rm'].
+      rewrite /allow_unlock_impl /has_lock_st /active_st. simpl.  
+      destruct decide. 
+      2: { simpl. trans False.
+           - apply neg_false. intros AL. inversion AL. by subst.
+           - symmetry. apply neg_false.
+             intros ([=]&?&?). subst. destruct H4.
+             destruct H3 as [? R]. rewrite R in n.
+             destruct x; [| set_solver]. eauto. }
+      split.
+      - intros AL. inversion AL. subst.
+        repeat split; eauto.
+        2: { rewrite e. set_solver. }
+        f_equal. apply wf_PI. 
+      - intros ([=]&[?[=]]&?). subst. econstructor.
+        destruct x; [| done]. edestruct H5; eauto.
+    Qed.
 
+    Definition allow_lock_impl (ρ: fmrole tl_fair_model) (st: tl_st): tl_st.
+      destruct st as [o t rm wf]. 
+      destruct (decide (rm !! ρ = Some (tl_L, false))) as [R|]. 
+      2: { exact (mkTlSt o t rm wf). }
+      pose proof (allows_lock_step ρ t o rm R).
+      pose proof (allows_lock'_preserves_tl_state_wf _ _ _ H wf).
+      esplit. apply H0. 
+    Defined. 
+          
+    Lemma allows_lock_impl_spec ρ st:
+      forall st', allows_lock ρ st st' <-> 
+              (allow_lock_impl ρ st = st' /\ (can_lock_st ρ st /\ ¬ active_st ρ st)).
+    Proof.
+      destruct st as [o t rm]. intros [o' t' rm'].
+      rewrite /allow_unlock_impl /can_lock_st /active_st. simpl.  
+      destruct decide. 
+      2: { simpl. trans False.
+           - apply neg_false. intros AL. inversion AL. by subst.
+           - symmetry. apply neg_false.
+             intros ([=]&?&?). subst. destruct H4.
+             destruct H3 as [? R]. rewrite R in n.
+             destruct x; [| set_solver]. eauto. }
+      split.
+      - intros AL. inversion AL. subst.
+        repeat split; eauto.
+        2: { rewrite e. set_solver. }
+        f_equal. apply wf_PI. 
+      - intros ([=]&[?[=]]&?). subst. econstructor.
+        destruct x; [| done]. edestruct H5; eauto.
+    Qed.
+      
     Instance TLFairLock: @FairLock _ tl_FLP tl_FLE. 
     Proof.
       econstructor.
@@ -1239,7 +1362,7 @@ Section Model.
         3: { apply (has_lock_kept_others ρ false). }
         2: { done. }
         red. intros ?? ->.
-        apply Morphisms_Prop.and_iff_morphism; [done| ]. 
+        (* apply Morphisms_Prop.and_iff_morphism; [done| ].  *)
         destruct (role_map y !! ρ) eqn:R; rewrite !R. 
         2: { set_solver. }
         split.
@@ -1261,17 +1384,19 @@ Section Model.
         intros X [? Y]. by rewrite X in Y.
       - simpl. by intros * ?%active_st_enabled.
       - simpl. intros. eapply has_lock_unique; eauto.
-        admit.
       - simpl. rewrite /has_lock_st /can_lock_st.
         intros * [??] [??]. congruence.
-      - simpl. intros * AU. inversion AU; subst; repeat split. 
+      - simpl. 
+        intros * AU. 
+        destruct tl_st1 as [o1 t1 rm1 wf1], tl_st2 as [o2 t2 rm2 wf2]. 
+        inversion AU; subst; repeat split. 
         + red. rewrite LOCK. eauto.
         + rewrite /active_st. rewrite LOCK. set_solver.
         + red. simpl. rewrite lookup_insert. eauto.
         + red. simpl. rewrite lookup_insert. eauto.
       - red. intros.
         eapply tl_progress; eauto.
-    Admitted. 
+    Qed. 
 
   End ProgressProperties. 
 
